new nomenclature... - ghost directory is now specs. - subtrace is now actor. - trace is now system.

src/specs/actor.fst
@@ -15,26 +15,29 @@
 
 //@requires "seq.fst"
 
-module Tesseract.Ghost.Subtrace
-
-   type step_g (state_t: Type) (event_t: Type) = 
-      | Init: state: state_t -> step_g state_t event_t
-      | Next: state: state_t -> event: event_t -> step_g state_t event_t
+module Tesseract.Specs.Actor
+   
+   type _step_g (state_t: Type) (event_t: Type) = 
+      | Spawn: state: state_t -> step_g state_t event_t
+      | Service: state: state_t -> event: event_t -> step_g state_t event_t
 
    type transform_g (state_t: Type) (event_t: Type) =
-      state_t -> event_t -> Tot state_t
+      state_t -> (state_t -> event_t) -> Tot state_t
 
-   type subtrace_g (state_t: Type) (event_t: Type) =
+   type actor_g (state_t: Type) (event_t: Type) =
       {
-         event_log: Seq.seq_g event_t;
+         event_log: Seq.seq_g (state_t -> event_t);
          transform: transform_g state_t event_t;
          state0: state_t
       }
 
-   val init: 
-      #state_t: Type -> #event_t: Type -> 
-      transform_g state_t event_t -> state_t -> Tot (subtrace_g state_t event_t)
-   let init (state_t: Type) (event_t: Type) f s = 
+   val spawn: 
+      #state_t: Type 
+      -> #event_t: Type
+      -> transform_g state_t event_t 
+      -> state_t 
+      -> Tot (actor_g state_t event_t)
+   let spawn (state_t: Type) (event_t: Type) f s = 
       {
          event_log = Seq.empty;
          transform = f;
@@ -42,26 +45,28 @@ module Tesseract.Ghost.Subtrace
       }
 
    val steps:
-      #state_t: Type -> #event_t: Type -> 
-      subtrace_g state_t event_t -> Tot (Seq.seq_g (step_g state_t event_t))
-   let steps (state_t: Type) (event_t: Type) subtrace =
-      let head = Seq.single (Init subtrace.state0) in
+      #state_t: Type 
+      -> #event_t: Type 
+      -> actor_g state_t event_t 
+      -> Tot (Seq.seq_g (step_g state_t (state_t -> event_t)))
+   let steps (state_t: Type) (event_t: Type) actor =
+      let head = Seq.single (Spawn actor.state0) in
       let tail =
          Seq.foldl
             (fun (accum: Seq.seq_g (step_g state_t event_t){0 < Seq.length accum}) event ->
                let step = 
                   (let state = 
                      match Seq.last accum with
-                        | Init s ->
+                        | Spawn s ->
                            s
-                        | Next s _ ->
+                        | Service s _ ->
                            s
                   in
-                     Next (subtrace.transform state event) event)
+                     Service (actor.transform state event) event)
                in
                   Seq.append accum step)
             head
-            subtrace.event_log
+            actor.event_log
       in
          Seq.concat head tail
 
